src/study/Nemonuri.Study.CSharpSyntaxRewriter2.Modifier2/Nemonuri.StratifiedNodes.Nodes.Children.fst
@@ -4,6 +4,7 @@ module L = FStar.List.Tot
 module Math = FStar.Math.Lib
 module I = Nemonuri.StratifiedNodes.Internals
 module T = Nemonuri.StratifiedNodes.Nodes.Base.Types
+module E = Nemonuri.StratifiedNodes.Nodes.Equivalence
 open Nemonuri.StratifiedNodes.Nodes.Base.Members
 open Nemonuri.StratifiedNodes.Nodes.Bijections
 
@@ -17,12 +18,19 @@ let get_children_length #t (node:T.node  t)
 //---|
 
 //--- private theory members ---
-let get_child_at #t (nd:T.node  t) (index:nat)
+let get_child_at #t (node:T.node t) (index:nat)
   : Pure (T.node  t) 
-    (requires (index < (get_children_length nd)))
-    (ensures fun r -> r = (L.index (get_children nd) index))
+    (requires (index < (get_children_length node)))
+    (ensures fun r -> r = (L.index (get_children node) index))
   =
+  let node_internal = I.get_item node.internal.children index in (
+    //assume ((L.index (get_children node) index).level = (I.get_level node_internal));
+    //assume ((L.index (get_children node) index).internal = node_internal);
+    assume ( E.are_equivalent_as_node_list_entails_get_item_pair_are_equivalent_as_node
+    (get_children node) (node.internal.children) index );
+    to_node node_internal
+  )
   // TODO: Internals 단계에서 구현하기
-  L.index (get_children nd) index
+  //L.index (get_children nd) index
 
 //---|
