src/study/Nemonuri.Study.CSharpSyntaxRewriter2.Modifier2/Nemonuri.StratifiedNodes.Nodes.Equivalence.fst
@@ -1,0 +1,60 @@
+module Nemonuri.StratifiedNodes.Nodes.Equivalence
+
+module L = FStar.List.Tot
+module I = Nemonuri.StratifiedNodes.Internals
+module N = Nemonuri.StratifiedNodes.Nodes.Base
+open Nemonuri.StratifiedNodes.Nodes.Bijections
+
+//--- theory members ---
+
+let are_equivalent_as_node #t #node_level 
+  (node:N.node t) (node_internal:I.node_internal t node_level)
+  : Tot bool =
+  (to_node node_internal = node)
+
+let are_equivalent_as_node_list #t #node_list_level
+  (node_list:N.node_list t) (node_list_internal:I.node_list_internal t node_list_level)
+  : Pure bool True
+    (ensures fun b -> 
+      if b then 
+        (L.length node_list) = (I.get_length node_list_internal)
+      else true
+    )
+  =
+  (to_node_list node_list_internal = node_list)
+
+//---|
+
+//--- propositions ---
+
+let are_equivalent_as_node_list_entails_get_item_pair_are_equivalent_as_node
+  #t #node_list_level
+  (node_list:N.node_list t) 
+  (node_list_internal:I.node_list_internal t node_list_level)
+  (index:nat)
+  : prop =
+  ((are_equivalent_as_node_list node_list node_list_internal) /\
+  (index < (L.length node_list))) ==>
+  (are_equivalent_as_node 
+    (L.index node_list index) (I.get_item node_list_internal index))
+
+//---|
+
+//--- lemma ---
+
+(*
+let lemma_are_equivalent_as_node_list_entails_get_item_pair_are_equivalent_as_node
+  #t #node_list_level
+  (node_list:N.node_list t) 
+  (node_list_internal:I.node_list_internal t node_list_level)
+  (index:nat)
+  : Lemma 
+    (requires (are_equivalent_as_node_list node_list node_list_internal) /\
+      (index < (L.length node_list)))
+    (ensures (are_equivalent_as_node 
+      (L.index node_list index) (I.get_item node_list_internal index)))
+  =
+  ()
+*)
+
+//---|
