src/study/Nemonuri.Study.CSharpSyntaxRewriter2.Modifier2/category.md
@@ -1,0 +1,31 @@
+# Category
+
+- node
+- node_internal
+
+## Object
+
+|| node | node_internal |
+| --- | --- | --- |
+| Alias | N | I |
+| Node type constructor | node: *t* → Type | node_internal: *t* → (node_level: pos) → Type |
+| Node list type constructor | node_list: *t* → Type | node_list_internal: *t* → (node_list_level: nat) → Type |
+| Node level getter | get_level: *t* → (node t) → pos | get_level: *t* → (node_level: pos) → (node_internal t pos) → (r:pos{r = node_level}) |
+| Empty node list constructor | *t* → (_: node_list t{Nil? _}) | *t* → (node_list_internal 0) |
+| Leaf node constructor | | |
+
+## Functor
+
+|| node → node_internal | node_internal → node | note |
+| --- | --- | --- | --- |
+| Node mapping | to_node_inverse: *t* → (n: N.node t) → (I.node_internal t (N.get_level n) ) | to_node: *t* → (node_level: pos) -> (I.node_internal t node_level) -> (N.node t) | fully faithful functors pair |
+
+## Axiom
+
+
+
+## Reference link
+
+- [Category (mathematics)](https://en.wikipedia.org/wiki/Category_(mathematics))
+- [Functor](https://en.wikipedia.org/wiki/Functor)
+- [Full and faithful functors](https://en.wikipedia.org/wiki/Full_and_faithful_functors)
